proofs/x86-64/avx2/ml_dsa_65/hashing_4x.ec
@@ -1,0 +1,264 @@
+require import AllCore IntDiv List.
+
+from Jasmin require import JModel_x86.
+
+from JazzEC require import Ml_dsa_65_avx2.
+
+from Spec require import GFq Rq Serialization Conversion Parameters VecMat Symmetric Sampling MLDSA_W32_Rep MLDSA.
+import PolyLVec PolyKVec PolyMat.
+import CDR Round Zq PolyReduceZq BigZMod.
+
+require import Array2 Array4 Array32 Array64 Array136 Array168.
+require import WArray2 WArray32 WArray64 WArray136 WArray168.
+
+(****************************************************************************)
+(* Clone KeccakArrayAvx2x4 for each array size used in hashing_4x.jinc     *)
+(* (Keccak1600_fixedsizes_avx2x4 re-exports Keccak1600_avx2x4, so          *)
+(*  absorb_spec_avx2x4 and Keccak1600_Jazz.M are available from here)       *)
+(****************************************************************************)
+
+from Keccak require import Keccak1600_fixedsizes_avx2x4.
+
+(****************************************************************************)
+(* Establish that M's 4x keccak primitives equal Keccak1600_Jazz.M          *)
+(****************************************************************************)
+
+equiv state_init_avx2x4_eq:
+ M.__state_init_avx2x4 ~ Keccak1600_Jazz.M.__state_init_avx2x4
+ : ={arg} ==> ={res}
+ by sim.
+
+equiv keccakf1600_avx2x4_eq:
+ M._keccakf1600_avx2x4 ~ Keccak1600_Jazz.M._keccakf1600_avx2x4
+ : ={arg} ==> ={res}
+ by sim.
+
+clone KeccakArrayAvx2x4 as A2avx2x4
+ with op _ASIZE <- 2,
+      theory A <- Array2,
+      theory WA <- WArray2
+      proof _ASIZE_ge0 by done
+      proof _ASIZE_u64 by done.
+
+clone KeccakArrayAvx2x4 as A32avx2x4
+ with op _ASIZE <- 32,
+      theory A <- Array32,
+      theory WA <- WArray32
+      proof _ASIZE_ge0 by done
+      proof _ASIZE_u64 by done.
+
+clone KeccakArrayAvx2x4 as A64avx2x4
+ with op _ASIZE <- 64,
+      theory A <- Array64,
+      theory WA <- WArray64
+      proof _ASIZE_ge0 by done
+      proof _ASIZE_u64 by done.
+
+clone KeccakArrayAvx2x4 as A136avx2x4
+ with op _ASIZE <- 136,
+      theory A <- Array136,
+      theory WA <- WArray136
+      proof _ASIZE_ge0 by done
+      proof _ASIZE_u64 by done.
+
+clone KeccakArrayAvx2x4 as A168avx2x4
+ with op _ASIZE <- 168,
+      theory A <- Array168,
+      theory WA <- WArray168
+      proof _ASIZE_ge0 by done
+      proof _ASIZE_u64 by done.
+
+(****************************************************************************)
+(* Equiv lemmas: M.primitive ~ KeccakArray.MM.primitive                     *)
+(****************************************************************************)
+
+equiv a2__absorb_avx2x4_eq:
+ M.a2____absorb_avx2x4 ~ A2avx2x4.MM.__absorb_avx2x4
+ : ={arg} ==> ={res}
+ by sim.
+
+equiv a32__absorb_bcast_avx2x4_eq:
+ M.a32____absorb_bcast_avx2x4 ~ A32avx2x4.MM.__absorb_bcast_avx2x4
+ : ={arg} ==> ={res}
+ by sim.
+
+equiv a64__absorb_bcast_avx2x4_eq:
+ M.a64____absorb_bcast_avx2x4 ~ A64avx2x4.MM.__absorb_bcast_avx2x4
+ : ={arg} ==> ={res}
+ by sim.
+
+equiv a136__dumpstate_avx2x4_eq:
+ M.a136____dumpstate_avx2x4 ~ A136avx2x4.MM.__dumpstate_avx2x4
+ : ={arg} ==> ={res}
+ by sim.
+
+equiv a168__dumpstate_avx2x4_eq:
+ M.a168____dumpstate_avx2x4 ~ A168avx2x4.MM.__dumpstate_avx2x4
+ : ={arg} ==> ={res}
+ by sim.
+
+(****************************************************************************)
+(* Module K: keccak-library wrapper mirroring M's 4x hashing procedures     *)
+(****************************************************************************)
+
+module K = {
+
+  proc shake128_absorb_34_4x (state:W256.t Array25.t, rho:W8.t Array32.t,
+                              domain_separators:W16.t Array4.t) :
+  W256.t Array25.t = {
+    var d0:W8.t Array2.t;
+    var d1:W8.t Array2.t;
+    var d2:W8.t Array2.t;
+    var d3:W8.t Array2.t;
+    var  _0:int;
+    var  _1:int;
+    d0 <- witness;
+    d1 <- witness;
+    d2 <- witness;
+    d3 <- witness;
+    state <@ Keccak1600_Jazz.M.__state_init_avx2x4 (state);
+    (state,  _0) <@ A32avx2x4.MM.__absorb_bcast_avx2x4 (state, 0, rho, 0, 168);
+    d0 <-
+    (Array2.init
+    (WArray2.get8
+    (WArray2.set16 (WArray2.init8 (fun i => d0.[i])) 0 domain_separators.[0])
+    ));
+    d1 <-
+    (Array2.init
+    (WArray2.get8
+    (WArray2.set16 (WArray2.init8 (fun i => d1.[i])) 0 domain_separators.[1])
+    ));
+    d2 <-
+    (Array2.init
+    (WArray2.get8
+    (WArray2.set16 (WArray2.init8 (fun i => d2.[i])) 0 domain_separators.[2])
+    ));
+    d3 <-
+    (Array2.init
+    (WArray2.get8
+    (WArray2.set16 (WArray2.init8 (fun i => d3.[i])) 0 domain_separators.[3])
+    ));
+    (state,  _1) <@ A2avx2x4.MM.__absorb_avx2x4 (state, 32, d0, d1, d2, d3, 31, 168);
+    return state;
+  }
+
+  proc shake256_absorb_66_4x (state:W256.t Array25.t,
+                              rho_prime:W8.t Array64.t,
+                              starting_domain_separator:W16.t) :
+  W256.t Array25.t = {
+    var t:W16.t;
+    var d0:W8.t Array2.t;
+    var d1:W8.t Array2.t;
+    var d2:W8.t Array2.t;
+    var d3:W8.t Array2.t;
+    var  _0:int;
+    var  _1:int;
+    d0 <- witness;
+    d1 <- witness;
+    d2 <- witness;
+    d3 <- witness;
+    state <@ Keccak1600_Jazz.M.__state_init_avx2x4 (state);
+    (state,  _0) <@ A64avx2x4.MM.__absorb_bcast_avx2x4 (state, 0, rho_prime, 0, 136);
+    t <- starting_domain_separator;
+    d0 <-
+    (Array2.init
+    (WArray2.get8 (WArray2.set16 (WArray2.init8 (fun i => d0.[i])) 0 t)));
+    t <- (t + (W16.of_int 1));
+    d1 <-
+    (Array2.init
+    (WArray2.get8 (WArray2.set16 (WArray2.init8 (fun i => d1.[i])) 0 t)));
+    t <- (t + (W16.of_int 1));
+    d2 <-
+    (Array2.init
+    (WArray2.get8 (WArray2.set16 (WArray2.init8 (fun i => d2.[i])) 0 t)));
+    t <- (t + (W16.of_int 1));
+    d3 <-
+    (Array2.init
+    (WArray2.get8 (WArray2.set16 (WArray2.init8 (fun i => d3.[i])) 0 t)));
+    (state,  _1) <@ A2avx2x4.MM.__absorb_avx2x4 (state, 64, d0, d1, d2, d3, 31, 136);
+    return state;
+  }
+
+  proc shake128_squeezeblock4x (state:W256.t Array25.t,
+                                h0:W8.t Array168.t, h1:W8.t Array168.t,
+                                h2:W8.t Array168.t, h3:W8.t Array168.t) :
+  W256.t Array25.t * W8.t Array168.t * W8.t Array168.t *
+  W8.t Array168.t * W8.t Array168.t = {
+    var offset:int;
+    var  _0:int;
+    state <@ Keccak1600_Jazz.M._keccakf1600_avx2x4 (state);
+    offset <- 0;
+    (h0, h1, h2, h3,  _0) <@ A168avx2x4.MM.__dumpstate_avx2x4 (h0, h1, h2, h3,
+    offset, 168, state);
+    return (state, h0, h1, h2, h3);
+  }
+
+  proc shake256_squeezeblock4x (state:W256.t Array25.t,
+                                h0:W8.t Array136.t, h1:W8.t Array136.t,
+                                h2:W8.t Array136.t, h3:W8.t Array136.t) :
+  W256.t Array25.t * W8.t Array136.t * W8.t Array136.t *
+  W8.t Array136.t * W8.t Array136.t = {
+    var offset:int;
+    var  _0:int;
+    state <@ Keccak1600_Jazz.M._keccakf1600_avx2x4 (state);
+    offset <- 0;
+    (h0, h1, h2, h3,  _0) <@ A136avx2x4.MM.__dumpstate_avx2x4 (h0, h1, h2, h3,
+    offset, 136, state);
+    return (state, h0, h1, h2, h3);
+  }
+
+}.
+
+(****************************************************************************)
+(* Equiv lemmas: M.proc ~ K.proc                                            *)
+(****************************************************************************)
+
+equiv shake128_absorb_34_4x_eq:
+ M.shake128_absorb_34_4x ~ K.shake128_absorb_34_4x
+ : ={arg} ==> ={res}
+ by sim.
+
+equiv shake256_absorb_66_4x_eq:
+ M.shake256_absorb_66_4x ~ K.shake256_absorb_66_4x
+ : ={arg} ==> ={res}
+ by sim.
+
+equiv shake128_squeezeblock4x_eq:
+ M.shake128_squeezeblock4x ~ K.shake128_squeezeblock4x
+ : ={arg} ==> ={res}
+ by sim.
+
+equiv shake256_squeezeblock4x_eq:
+ M.shake256_squeezeblock4x ~ K.shake256_squeezeblock4x
+ : ={arg} ==> ={res}
+ by sim.
+
+(****************************************************************************)
+(* Correctness lemmas (absorbed-state characterization)                     *)
+(****************************************************************************)
+
+phoare shake128_absorb_34_4x_ph _rho _ds :
+ [ M.shake128_absorb_34_4x
+ : arg.`2 = _rho /\ arg.`3 = _ds
+ ==>
+   absorb_spec_avx2x4 168 31
+     (to_list _rho ++ to_list (Array2.init (WArray2.get8 (WArray2.set16 (WArray2.init8 (fun i => witness)) 0 _ds.[0]))))
+     (to_list _rho ++ to_list (Array2.init (WArray2.get8 (WArray2.set16 (WArray2.init8 (fun i => witness)) 0 _ds.[1]))))
+     (to_list _rho ++ to_list (Array2.init (WArray2.get8 (WArray2.set16 (WArray2.init8 (fun i => witness)) 0 _ds.[2]))))
+     (to_list _rho ++ to_list (Array2.init (WArray2.get8 (WArray2.set16 (WArray2.init8 (fun i => witness)) 0 _ds.[3]))))
+     res
+ ] = 1%r.
+admitted.
+
+phoare shake256_absorb_66_4x_ph _rho_prime _ds0 :
+ [ M.shake256_absorb_66_4x
+ : arg.`2 = _rho_prime /\ arg.`3 = _ds0
+ ==>
+   absorb_spec_avx2x4 136 31
+     (to_list _rho_prime ++ to_list (Array2.init (WArray2.get8 (WArray2.set16 (WArray2.init8 (fun i => witness)) 0 _ds0))))
+     (to_list _rho_prime ++ to_list (Array2.init (WArray2.get8 (WArray2.set16 (WArray2.init8 (fun i => witness)) 0 (_ds0 + W16.one)))))
+     (to_list _rho_prime ++ to_list (Array2.init (WArray2.get8 (WArray2.set16 (WArray2.init8 (fun i => witness)) 0 (_ds0 + (W16.of_int 2))))))
+     (to_list _rho_prime ++ to_list (Array2.init (WArray2.get8 (WArray2.set16 (WArray2.init8 (fun i => witness)) 0 (_ds0 + (W16.of_int 3))))))
+     res
+ ] = 1%r.
+admitted.
